dimsum_examples/compiler/compiler.v
@@ -5,6 +5,9 @@ From dimsum.examples.compiler Require Import monad linear_imp ssa linearize mem2
 Local Open Scope Z_scope.
 Set Default Proof Using "Type".
 
+(** * Compiler from Imp to Asm  *)
+
+(** * Helper lemmas  *)
 Lemma tmp_var_ne_ssa_var n1 s n2 :
   tmp_var n1 ≠ ssa_var s n2.
 Proof.
@@ -14,6 +17,7 @@ Proof.
   rewrite pretty_N_last /pretty_N_char. by repeat case_match.
 Qed.
 
+(** * Definition of the compiler  *)
 Inductive compile_error :=
 | LinearizeError (e : ci2a_linearize.error)
 | CodegenError (e : ci2a_codegen.error)
@@ -34,7 +38,14 @@ Definition compile (f2i : gmap string Z) (fn : fndef) : compiler_success compile
   opt ← compile_mem2reg fn;
   compiler_success_fmap_error CodegenError (ci2a_codegen.pass_fn f2i opt).
 
-Lemma compile_correct f2i f fn dins ins a:
+Ltac i2a_compile f2i f :=
+  (let e := eval vm_compute in
+      match compile f2i f with
+      | monad.CSuccess i => i | monad.CError _ => [] end
+   in exact e).
+
+(** * Compiler correctness proof  *)
+Theorem compile_correct f2i f fn dins ins a:
   compile f2i fn = CSuccess dins →
   ins = deep_to_asm_instrs a dins →
   f2i !! f = Some a →
@@ -71,12 +82,7 @@ Proof.
   done.
 Qed.
 
-Ltac i2a_compile f2i f :=
-  (let e := eval vm_compute in
-      match compile f2i f with
-      | monad.CSuccess i => i | monad.CError _ => [] end
-   in exact e).
-
+(** * Tests *)
 Module ci2a_test.
 
 Definition test_fn_1 : fndef := {|
@@ -86,10 +92,62 @@ Definition test_fn_1 : fndef := {|
   fd_static := I;
 |}.
 
-Compute compile_ssa test_fn_1.
-Compute compile_linear test_fn_1.
-Compute compile_mem2reg test_fn_1.
-Compute compile (<["f" := 100]> ∅) test_fn_1.
+Lemma test :
+ compile_ssa test_fn_1 =
+ {|
+    sfd_args := ["x$0"];
+    sfd_vars := [("y$1", 1)];
+    sfd_body :=
+      SBinOp (SBinOp (SVar "x$0") ShiftOp (SVal (StaticValNum 2))) AddOp
+        (SCall "f" [SLoad (SVar "x$0"); SLoad (SVar "y$1"); SVal (StaticValNum 1)])
+ |}.
+Proof. vm_compute. match goal with |- ?x = ?x => idtac end. Abort.
+
+Lemma test :
+ compile_linear test_fn_1 =
+  CSuccess {|
+      lfd_args := ["x$0"];
+      lfd_vars := [("y$1", 1)];
+      lfd_body :=
+        LLetE "$0$" (LBinOp (VVar "x$0") ShiftOp (VVal (StaticValNum 2)))
+          (LLetE "$1$" (LLoad (VVar "x$0"))
+             (LLetE "$2$" (LLoad (VVar "y$1"))
+                (LLetE "$3$" (LCall "f" [VVar "$1$"; VVar "$2$"; VVal (StaticValNum 1)])
+                   (LLetE "$4$" (LBinOp (VVar "$0$") AddOp (VVar "$3$")) (LEnd (LVarVal (VVar "$4$")))))))
+  |}.
+Proof. vm_compute. match goal with |- ?x = ?x => idtac end. Abort.
+
+Lemma test :
+ compile_mem2reg test_fn_1 =
+  CSuccess
+    {|
+      lfd_args := ["x$0"];
+      lfd_vars := [];
+      lfd_body :=
+        LLetE "y$1" (LVarVal (VVal (StaticValNum 0)))
+          (LLetE "$0$" (LBinOp (VVar "x$0") ShiftOp (VVal (StaticValNum 2)))
+             (LLetE "$1$" (LLoad (VVar "x$0"))
+                (LLetE "$2$" (LVarVal (VVar "y$1"))
+                   (LLetE "$3$" (LCall "f" [VVar "$1$"; VVar "$2$"; VVal (StaticValNum 1)])
+                      (LLetE "$4$" (LBinOp (VVar "$0$") AddOp (VVar "$3$")) (LEnd (LVarVal (VVar "$4$"))))))))
+    |}.
+Proof. vm_compute. match goal with |- ?x = ?x => idtac end. Abort.
+
+Lemma test :
+ compile (<["f" := 100]> ∅) test_fn_1 =
+  CSuccess
+    [Aload "R17" "SP" (-1); Astore "R30" "SP" (-1); Aload "R17" "SP" (-2); Astore "R19" "SP" (-2);
+    Aload "R17" "SP" (-3); Astore "R20" "SP" (-3); Aload "R17" "SP" (-4); Astore "R21" "SP" (-4);
+    Aload "R17" "SP" (-5); Astore "R22" "SP" (-5); Aload "R17" "SP" (-6); Astore "R23" "SP" (-6);
+    Aload "R17" "SP" (-7); Astore "R24" "SP" (-7); Aload "R17" "SP" (-8); Astore "R25" "SP" (-8);
+    Amov "R19" "R0"; Aadd "SP" "SP" (-8); Amov "R0" 0; Amov "R20" "R0"; Amov "R1" "R19";
+    Amov "R2" 2; Aadd "R0" "R1" "R2"; Amov "R21" "R0"; Amov "R1" "R19"; Aload "R0" "R1" 0;
+    Amov "R22" "R0"; Amov "R0" "R20"; Amov "R23" "R0"; Amov "R0" "R22"; Amov "R1" "R23";
+    Amov "R2" 1; Abranch_link true 100; Amov "R24" "R0"; Amov "R1" "R21"; Amov "R2" "R24";
+    Aadd "R0" "R1" "R2"; Amov "R25" "R0"; Amov "R0" "R25"; Aadd "SP" "SP" 8; Aload "R25" "SP" (-8);
+    Aload "R24" "SP" (-7); Aload "R23" "SP" (-6); Aload "R22" "SP" (-5); Aload "R21" "SP" (-4);
+    Aload "R20" "SP" (-3); Aload "R19" "SP" (-2); Aload "R30" "SP" (-1); Aret].
+Proof. vm_compute. match goal with |- ?x = ?x => idtac end. Abort.
 
 Definition test_sum : fndef := {|
   fd_args := ["n"];
@@ -103,7 +161,51 @@ Definition test_sum : fndef := {|
   fd_static := I;
 |}.
 
-Compute compile_ssa test_sum.
-Compute compile_linear test_sum.
-Compute compile (<["sum" := 100]> ∅) test_sum.
+Lemma test :
+ compile_ssa test_sum =
+ {|
+    sfd_args := ["n$0"];
+    sfd_vars := [];
+    sfd_body :=
+      SIf (SBinOp (SVar "n$0") EqOp (SVal (StaticValNum 0))) (SVal (StaticValNum 0))
+        (SLetE "rec$1" (SCall "sum" [SBinOp (SVar "n$0") AddOp (SVal (StaticValNum (-1)))])
+           (SBinOp (SVar "n$0") AddOp (SVar "rec$1")))
+  |}.
+Proof. vm_compute. match goal with |- ?x = ?x => idtac end. Abort.
+
+Lemma test :
+ compile_linear test_sum =
+ CSuccess
+    {|
+      lfd_args := ["n$0"];
+      lfd_vars := [];
+      lfd_body :=
+        LLetE "$0$" (LBinOp (VVar "n$0") EqOp (VVal (StaticValNum 0)))
+          (LIf (LVarVal (VVar "$0$"))
+             (LLetE "$4$" (LVarVal (VVal (StaticValNum 0))) (LEnd (LVarVal (VVar "$4$"))))
+             (LLetE "$1$" (LBinOp (VVar "n$0") AddOp (VVal (StaticValNum (-1))))
+                (LLetE "$2$" (LCall "sum" [VVar "$1$"])
+                   (LLetE "rec$1" (LVarVal (VVar "$2$"))
+                      (LLetE "$3$" (LBinOp (VVar "n$0") AddOp (VVar "rec$1"))
+                         (LLetE "$4$" (LVarVal (VVar "$3$")) (LEnd (LVarVal (VVar "$4$")))))))))
+    |}.
+Proof. vm_compute. match goal with |- ?x = ?x => idtac end. Abort.
+
+Lemma test :
+ compile (<["sum" := 100]> ∅) test_sum =
+  CSuccess
+    [Aload "R17" "SP" (-1); Astore "R30" "SP" (-1); Aload "R17" "SP" (-2); Astore "R19" "SP" (-2);
+    Aload "R17" "SP" (-3); Astore "R20" "SP" (-3); Aload "R17" "SP" (-4); Astore "R21" "SP" (-4);
+    Aload "R17" "SP" (-5); Astore "R22" "SP" (-5); Aload "R17" "SP" (-6); Astore "R23" "SP" (-6);
+    Aload "R17" "SP" (-7); Astore "R24" "SP" (-7); Aload "R17" "SP" (-8); Astore "R25" "SP" (-8);
+    Amov "R19" "R0"; Aadd "SP" "SP" (-8); Amov "R1" "R19"; Amov "R2" 0; Aseq "R0" "R1" "R2";
+    Amov "R20" "R0"; Amov "R0" "R20"; Abranch_eq false 5 "R0" 0; Amov "R0" 0; Amov "R25" "R0";
+    Amov "R0" "R25"; Abranch false 17; Amov "R1" "R19"; Amov "R2" (-1); Aadd "R0" "R1" "R2";
+    Amov "R21" "R0"; Amov "R0" "R21"; Abranch_link true 100; Amov "R22" "R0"; Amov "R0" "R22";
+    Amov "R23" "R0"; Amov "R1" "R19"; Amov "R2" "R23"; Aadd "R0" "R1" "R2"; Amov "R24" "R0";
+    Amov "R0" "R24"; Amov "R25" "R0"; Amov "R0" "R25"; Aadd "SP" "SP" 8; Aload "R25" "SP" (-8);
+    Aload "R24" "SP" (-7); Aload "R23" "SP" (-6); Aload "R22" "SP" (-5); Aload "R21" "SP" (-4);
+    Aload "R20" "SP" (-3); Aload "R19" "SP" (-2); Aload "R30" "SP" (-1); Aret].
+Proof. vm_compute. match goal with |- ?x = ?x => idtac end. Abort.
+
 End ci2a_test.
