dimsum_examples/compiler/linear_imp.v
@@ -1,5 +1,9 @@
 From dimsum.examples Require Export imp.
 
+(** * Linear Imp *)
+(** This file defines a linear subset of Imp, corresponding to the A-normal form. *)
+
+(** * Variables or Values *)
 Inductive var_val :=
 | VVar (v : string)
 | VVal (v : static_val).
@@ -35,6 +39,11 @@ Lemma lookup_var_val_mono vs vs' v v':
   lookup_var_val vs' v = Some v'.
 Proof. destruct v => //. simplify_eq/=. apply lookup_weaken. Qed.
 
+Lemma var_val_is_static v :
+  is_static_expr false (var_val_to_expr v).
+Proof. destruct v => //=. by destruct v. Qed.
+
+(** * Operations *)
 Inductive lexpr_op :=
 | LVarVal (v : var_val)
 | LBinOp (v1 : var_val) (o : binop) (v2 : var_val)
@@ -51,6 +60,14 @@ Definition lexpr_op_to_expr (e : lexpr_op) : expr :=
   | LCall f args => Call f (var_val_to_expr <$> args)
   end.
 
+Lemma lexpr_op_is_static e :
+  is_static_expr false (lexpr_op_to_expr e).
+Proof.
+  destruct e => //=; rewrite ?andb_True; split!; try apply var_val_is_static.
+  apply forallb_True. rewrite Forall_fmap. apply Forall_true => ?. apply var_val_is_static.
+Qed.
+
+(** * Expressions *)
 Inductive lexpr :=
 | LLetE (v : string) (e1 : lexpr_op) (e2 : lexpr)
 | LIf (e1 : lexpr_op) (e2 e3 : lexpr)
@@ -63,21 +80,11 @@ Fixpoint lexpr_to_expr (e : lexpr) : expr :=
   | LEnd e => (lexpr_op_to_expr e)
   end.
 
-Lemma var_val_is_static v :
-  is_static_expr false (var_val_to_expr v).
-Proof. destruct v => //=. by destruct v. Qed.
-
-Lemma lexpr_op_is_static e :
-  is_static_expr false (lexpr_op_to_expr e).
-Proof.
-  destruct e => //=; rewrite ?andb_True; split!; try apply var_val_is_static.
-  apply forallb_True. rewrite Forall_fmap. apply Forall_true => ?. apply var_val_is_static.
-Qed.
-
 Lemma lexpr_is_static e :
   is_static_expr false (lexpr_to_expr e).
 Proof. elim: e => //= *; rewrite ?andb_True; split!; apply lexpr_op_is_static. Qed.
 
+(** * Function declarations *)
 Record lfndef : Type := {
   lfd_args : list string;
   lfd_vars : list (string * Z);
